eve/Src/framework/eiffel2boogie/e2b_messages.e
@@ -13,7 +13,7 @@ inherit
 feature -- Validity error messages
 
 	functional_feature_not_function: STRING_32
-		do Result := "Functional feature has to be a function." end
+		do Result := "Functional feature has to be a pure function." end
 
 	functional_feature_not_single_assignment: STRING_32
 		do Result := "A functional feature has to consist of exactly one assignment to the Result." end
@@ -41,6 +41,9 @@ feature -- Validity error messages
 
 	invalid_context_for_special_predicate (a_kind: STRING): STRING_32
 		do Result := locale.formatted_string ("$1 clauses are only allowed in preconditions and loop invariants (will be ignored)", a_kind) end
+
+	invalid_context_for_read_predicate: STRING_32
+		do Result := "Read sets are only allowed for functions (will be ignored)" end
 
 	variant_bad_type (a_index: INTEGER): STRING_32
 		do Result := locale.formatted_string ("Type of variant number $1 has no well-founded order.", a_index.out) end
@@ -101,8 +104,8 @@ feature -- Verification error messages
 	decreases_not_decreasing: STRING_32
 		do Result := "Variant may not decrease at this recursive call / the end of this loop body." end
 
-	decreases_bounded (index: STRING): STRING_32
-		do Result := locale.formatted_string ("Integer variant component at position $1 may be negative.", index) end
+	decreases_bounded: STRING_32
+		do Result := "Integer variant component at position $variant may be negative." end
 
 	overflow: STRING_32
 		do Result := "Possible arithmetic overflow." end
@@ -132,7 +135,13 @@ feature -- Verification error messages
 		do Result := "Observers of the assignment target may be invalidated." end
 
 	assignment_attribute_writable: STRING_32
-		do Result := "The attribute of the assignment may not be writable." end
+		do Result := "Target attribute may not be writable." end
+
+	access_attribute_readable: STRING_32
+		do Result := "Attribute $called_feature might not be readable." end
+
+	access_frame_readable: STRING_32
+		do Result := "Some memebers of the read frame of $called_feature might not be readable." end
 
 	ownership_explicit_note: STRING_32
 		do Result := "Disable this default by making $explicit_value explicit." end
