eve/Src/framework/eiffel2boogie/translation/pool/e2b_tu_read_frame.e
@@ -1,12 +1,12 @@
 note
 	description: "[
-		Translation unit for the frame function of an Eiffel routine.
+		Translation unit for the read frame function of an Eiffel function.
 	]"
 	date: "$Date$"
 	revision: "$Revision$"
 
 class
-	E2B_TU_FRAME
+	E2B_TU_READ_FRAME
 
 inherit
 
@@ -17,7 +17,7 @@ create
 
 feature -- Access
 
-	base_id: STRING = "writes-function"
+	base_id: STRING = "read-frame"
 			-- <Precursor>
 
 feature -- Basic operations
@@ -28,7 +28,6 @@ feature -- Basic operations
 			l_translator: E2B_ROUTINE_TRANSLATOR
 		do
 			create l_translator.make
-			l_translator.translate_frame_function (feat, type)
+			l_translator.translate_frame_function (feat, type, True)
 		end
-
 end
